\section{Séries de Fourier}

\subsection{Produto interno de funcões - revisão}
\begin{boxedeq}[0.4]
    \left\langle f, g \right\rangle = \int_{-\frac{T}{2}}^{\frac{T}{2}} f(x) \overline{g(x)}\,dt
\end{boxedeq}

\subsection{Séries de Fourier}
\subsubsection{Forma exponencial complexa}
\begin{boxedeq}[0.3]
    f(t) = \sum_{n=-\infty}^{\infty} c_n e^{i n \omega t}
\end{boxedeq}
\begin{boxedeq}
    c_n = \frac{1}{T}\left\langle f, e^{i n \omega t} \right\rangle = \frac{1}{T} \int_{-\frac{T}{2}}^{\frac{T}{2}} f(t) e^{-i n \omega t} dt
\end{boxedeq}

\subsubsection{Forma trignométrica}
\begin{boxedeq}[0.6]
    f(t) = \frac{a_0}{2} + \sum_{k=1}^{\infty} \left[ a_k \cos(k \omega t) + b_k \sin(k \omega t) \right]
\end{boxedeq}
\begin{boxedeq}[0.4]
    \frac{a_0}{2} = c_0 = \frac{1}{T} \int_{-\frac{T}{2}}^{\frac{T}{2}} f(t) dt
\end{boxedeq}
\begin{boxedeq}
    a_k = c_k - c_{-k} = \frac{2}{T} \int_{-\frac{T}{2}}^{\frac{T}{2}} f(t) \cos(k \omega t) dt
\end{boxedeq}
\begin{boxedeq}
    b_n = i(c_k - c_{-k}) = \frac{2}{T} \int_{-\frac{T}{2}}^{\frac{T}{2}} f(t) \sin(k \omega t) dt
\end{boxedeq}