\documentclass{article}

\usepackage{graphicx}
\usepackage[portuguese]{babel}
\usepackage{indentfirst}
\usepackage{amsmath}
\usepackage[top=1in,bottom=1in,left=1in,right=1in]{geometry}
\usepackage{hyperref}

\title{Cálculo - III}
\author{Samuel Fortunato}

\begin{document}
\section{Produto interno de funcões - revisão}
\Large{
    \begin{gather*}
        \left\langle f, g \right\rangle = \int_{-\frac{T}{2}}^{\frac{T}{2}} f(x) \overline{g(x)}\,dt
    \end{gather*}
}

\section{Séries de Fourier}
\subsection{Forma exponencial complexa}
\Large{
    \begin{gather*}
        f(t) = \sum_{n=-\infty}^{\infty} c_n e^{i n \omega t} \\
        \\
        c_n = \frac{1}{T}\left\langle f, e^{i n \omega t} \right\rangle = \frac{1}{T} \int_{-\frac{T}{2}}^{\frac{T}{2}} f(t) e^{-i n \omega t} dt
    \end{gather*}
}

\subsection{Forma trignométrica}
\Large{
    \begin{gather*}
        f(t) = \frac{a_0}{2} + \sum_{k=1}^{\infty} \left[ a_k \cos(k \omega t) + b_k \sin(k \omega t) \right] \\
        \\
        \frac{a_0}{2} = c_0 = \frac{1}{T} \int_{-\frac{T}{2}}^{\frac{T}{2}} f(t) dt \\
        \\
        a_k = c_k - c_{-k} = \frac{2}{T} \int_{-\frac{T}{2}}^{\frac{T}{2}} f(t) \cos(k \omega t) dt \\
        \\
        b_n = i(c_k - c_{-k}) = \frac{2}{T} \int_{-\frac{T}{2}}^{\frac{T}{2}} f(t) \sin(k \omega t) dt 
    \end{gather*}
}

\end{document}